add inductive definitions, equivalence proof and show algebraic properties

CSL.v
@@ -15,24 +15,73 @@ match e1,e2 with
 | _ , _ => false
 end.
 
-(*For equality should I try with computational reflection as it
- is done in the libraries: https://coq.inria.fr/library/Coq.Bool.Sumbool.html
- and seen in software foundations: https://softwarefoundations.cis.upenn.edu/vfa-current/Decide.html*)
+Lemma eq_event_refl : forall e, eq_event e e = true.
+Proof. destruct e.
+- reflexivity.
+- reflexivity.
+Qed.
 
-(*Definition event_dec : forall a b : EventType, {a = b} + {a <> b}.*)
+Lemma eq_event_equals : forall (e1 e2 : EventType), (eq_event e1 e2) = true -> e1 = e2.
+Proof. intros e1 e2 H. destruct e1.
+  - simpl in H. destruct e2.
+    * reflexivity.
+    * discriminate.
+  - simpl in H. destruct e2.
+    * discriminate.
+    * reflexivity.
+Qed.
 
+Lemma equals_eq_event : forall (e1 e2 : EventType), e1 = e2 -> (eq_event e1 e2) = true.
+Proof. intros e1 e2 H. inversion H. apply eq_event_refl.
+Qed.
+
+Lemma eq_event_iff_eq : forall (e1 e2 : EventType), (eq_event e1 e2) = true <-> e1 = e2.
+Proof. split.
+- apply eq_event_equals.
+- apply equals_eq_event.
+Qed.
+
+Inductive reflect (P : Prop) : bool -> Prop :=
+| ReflectT (H :   P) : reflect P true
+| ReflectF (H : ~ P) : reflect P false.
+
+Theorem iff_reflect : forall P b, (P <-> b = true) -> reflect P b.
+Proof.
+  intros P b H. destruct b.
+  - apply ReflectT. rewrite H. reflexivity.
+  - apply ReflectF. rewrite H. intros H'. discriminate.
+Qed.
+
+Theorem reflect_iff : forall P b, reflect P b -> (P <-> b = true).
+Proof.
+intros P b H. inversion H.
+- split.
+  * intro H2. reflexivity.
+  * intro H2. apply H0.
+- split. intros H2. inversion H. rewrite <- H1 in H4. discriminate H4.
+  destruct b.
+  * discriminate.
+  * exfalso. unfold not in H3. apply H3 in H2. apply H2.
+  * intro H3. discriminate.
+Qed.
+
+Lemma eq_event_prop : forall n m, reflect (n = m) (eq_event n m).
+Proof.
+  intros n m. apply iff_reflect. split.
+- apply eq_event_iff_eq.
+- apply eq_event_iff_eq.
+Qed.
 
 Definition Trace := List.list EventType % type.
-
 
 Inductive Contract : Set :=
 | Success : Contract
 | Failure : Contract
-| Event : EventType -> Contract -> Contract
+| Event : EventType -> Contract
 | CPlus : Contract -> Contract -> Contract
 | CSeq : Contract -> Contract -> Contract.
 
-Notation "e _._ c" := (Event e c)
+Notation "e _._ c" := (CSeq (Event e) c)
                     (at level 41, right associativity).
 
 Notation "c0 _;_ c1"  := (CSeq c0 c1)
@@ -46,8 +95,8 @@ Fixpoint nu(c:Contract):bool :=
 match c with
 | Success => true
 | Failure => false
-| e _._ c => false
-| c0 _;_ c1 => nu c0
+| Event e => false
+| c0 _;_ c1 => nu c0 && nu c1
 | c0 _+_ c1 => nu c0 || nu c1
 end.
 
@@ -57,10 +106,10 @@ Fixpoint derive(e:EventType)(c:Contract):Contract :=
 match c with
 | Success => Failure
 | Failure => Failure
-| e1 _._ c => if eq_event e1 e then c else Failure
+| Event e1 => if eq_event e1 e then Success else Failure
 | c0 _;_ c1 => match nu c0 with
-               | true => (derive e c0) _+_ (derive e c1)
-               | false => (derive e c0)
+               | true => ((derive e c0) _;_ c1) _+_ (derive e c1)
+               | false => (derive e c0) _;_ c1
                end
 | c0 _+_ c1 => (derive e c0) _+_ (derive e c1)
 end.
@@ -75,41 +124,229 @@ match s with
 end.
 
 (*Expression*)
-Notation "c ~= s" := (matches c s) (at level 60).
+Notation "s =~ c" := (matches c s) (at level 62).
 
 (*Propositions*)
-Notation "c ~== s" := (matches c s = true) (at level 60).
-Notation "c ~!= s" := (matches c s = false) (at level 60).
+
+Notation "s !=~ c" := (matches c s = false) (at level 62).
 
 (** Relation between [matches] and [derive]. *)
 Theorem derivation : forall (e:EventType)(s:Trace)(c:Contract),
-  c ~= (e::s) = c / e ~= s.
-Proof. intros e s c. simpl. auto. 
+  (e::s) =~ c  = s =~ c / e.
+Proof. intros e s c. simpl. reflexivity.
 Qed.
 
-(*[Contract] as Setoid*)
-Definition c_eq (c c':Contract) : Prop := forall s, c ~= s = c' ~=s.
+Reserved Notation "s ==~ re" (at level 60).
 
-Check reflexive.
+Inductive exp_match : Trace -> Contract -> Prop :=
+  | MSuccess : [] ==~ Success
+  | MEvent x : [x] ==~ (Event x)
+  | MSeq s1 c1 s2 c2
+             (H1 : s1 ==~ c1)
+             (H2 : s2 ==~ c2)
+           : (s1 ++ s2) ==~ (c1 _;_ c2)
+  | MPlusL s1 c1 c2
+                (H1 : s1 ==~ c1)
+              : s1 ==~ (c1 _+_ c2)
+  | MPlusR c1 s2 c2
+                (H2 : s2 ==~ c2)
+              : s2 ==~ (c1 _+_ c2)
+  where "s ==~ c" := (exp_match s c).
 
+(* eq_event x x *)
+(*mseq at op level*)
+
+(*If s matches c, it also matches c _+_ any contract*)
+Lemma plus_left_oper : forall (s : Trace)(l r : Contract), s =~ l = true -> s =~ (l _+_ r) = true.
+Proof. intros s. induction s as [| n s' IHs'].
+- intros l r H. simpl in H. simpl. rewrite H. rewrite orb_true_l. reflexivity.
+- simpl. intros l r H. apply IHs'. apply H.
+Qed. 
+
+(*_+_ is commutative*)
+Lemma plus_comm_oper : forall (s : Trace)(l r : Contract), s =~ (l _+_ r) = true -> s =~ (r _+_ l) = true.
+Proof. induction s as [| e s' IHs'].
+- simpl. intros l r H. rewrite orb_comm. apply H.
+- intros l r H. simpl. apply IHs'. simpl in H. apply H.
+Qed.
+ 
+(*If s matches c, it also matches any contract _+_ c*)
+Lemma plus_right_oper : forall (s : Trace)(l r : Contract), s =~ r = true -> s =~ (l _+_ r) = true.
+Proof. intros s l r H. apply plus_comm_oper. apply plus_left_oper. apply H.
+Qed.
+
+(*If s matches c2, it will still match after prefixing c2 with a nullary contract*)
+Lemma seq_nu_left : forall (s : Trace)(c1 c2 : Contract), nu c1 = true -> (s =~c2 = true) 
+                    -> (s =~ c1 _;_ c2 = true).
+Proof. induction s as [| e s' IHs'].
+- intros c1 c2 H1 H2. unfold matches. simpl. simpl in H2. apply andb_true_intro.
+  split.
+  * apply H1.
+  * apply H2.
+- intros c1 c2 H1 H2. simpl. rewrite H1. simpl in H2. apply plus_right_oper. apply H2.
+Qed.
+
+(*MSeq defined operationally*)
+Lemma mseq_oper : forall (s1 s2 : Trace)(c1 c2 : Contract), s1 =~ c1 = true -> 
+                      s2 =~ c2 = true -> ((s1 ++ s2) =~ c1 _;_ c2) = true.
+Proof. induction s1 as [| e s1' IHs1'].
+- simpl. intros s2 c1 c2 H1 H2. rewrite <- (app_nil_l s2).
+  apply seq_nu_left.
+  * apply H1.
+  * simpl. apply H2.
+- intros s2 c1 c2 H1 H2. simpl. destruct (nu c1).
+  * simpl in H1. simpl in H1. rewrite <- (app_nil_l (s1' ++ s2)). apply plus_left_oper.
+    simpl. apply IHs1'.
+    ** apply H1.
+    ** apply H2.
+  * apply IHs1'.
+    ** simpl in H1. apply H1.
+    ** apply H2.
+Qed. 
+
+Lemma comp_imp_oper : forall (s : Trace)(c : Contract), s ==~ c -> (s =~ c) = true.
+Proof. 
+intros s c H. induction H.
+- simpl. reflexivity. (*MSucces*)
+- simpl. rewrite eq_event_refl. reflexivity. (*MChar*)
+- apply mseq_oper. (*MSeq*)
+  * apply IHexp_match1.
+  * apply IHexp_match2.   
+- apply plus_left_oper. apply IHexp_match.  (*MPlusL*)
+- apply plus_right_oper. apply IHexp_match. (*MPlusR*)
+Qed.
+
+(*No trace can be derived from Failure*)
+Lemma failure_false : forall (s : Trace), (s =~ Failure) = false.
+Proof. induction s.
+- simpl. reflexivity.
+- simpl. apply IHs.
+Qed.
+
+(*Only the empty trace can be derived from Success*)
+Lemma success_empty : forall (s : Trace), (s =~ Success) = true -> s = [].
+Proof. induction s.
+- intro H. reflexivity.
+- simpl. rewrite failure_false. intro H. discriminate.
+Qed.
+
+(*If s matches c1 _+_ c2, then it matches c1 or c2*)
+Lemma plus_or_oper : forall (s : Trace)(c1 c2 : Contract), (s =~ (c1 _+_ c2)) = true -> 
+               (s =~ c1) = true \/ (s =~ c2) = true.
+Proof. induction s.
+- intros c1 c2 H. simpl. simpl in H. apply orb_prop in H. apply H.
+- intros c1 c2 H. simpl. apply IHs. simpl in H. apply H.
+Qed.
+
+
+Definition exists_seq_decomp_def (s : Trace) (c1 c2 : Contract) : Prop := 
+ s =~ c1 _;_ c2 = true ->
+     exists s1 s2 : Trace, s = s1 ++ s2 /\ s1 =~ c1 = true /\ s2 =~ c2 = true.
+
+(*To show e::s matching c1 _;_ c2 can be decomposed, it suffices to show 
+  s matching c1/e ;_ c2 can be decomposed*)
+Lemma mseq_oper_inv_helper : forall (s : Trace)(c1 c2 : Contract)(e : EventType), 
+  (exists_seq_decomp_def s (c1 / e) c2) -> exists_seq_decomp_def (e :: s) c1 c2.
+Proof.
+unfold exists_seq_decomp_def. intros s c1 c2 e H1 H2. simpl in H2. destruct (nu c1) eqn:Heqn.
+- apply plus_or_oper in H2 as H2. destruct H2 as [H2 | H2].
+  * apply H1 in H2. destruct H2 as [s' [s'' [P1 [P2 P3]]]].
+    exists (e::s'). exists s''. simpl. rewrite P1. split.
+    ** reflexivity.
+    ** split. 
+      *** apply P2.
+      *** apply P3.
+  * exists []. exists (e::s). simpl. split.
+    ** reflexivity.
+    ** split. { apply Heqn. } { apply H2. }
+- apply H1 in H2. destruct H2 as [s' [s'' [P1 [P2 P3]]]]. exists (e::s'). exists s''. split.
+  * simpl. rewrite <- P1. reflexivity.
+  * split.
+    ** simpl. apply P2.
+    ** apply P3.
+Qed.
+
+
+
+
+(*The inverse rule of MSeq given operationally*)
+Lemma mseq_oper_inv : forall (s : Trace)(c1 c2 : Contract), 
+       (s =~ c1 _;_ c2) = true -> (exists (s1 s2 : Trace), s = s1++s2 /\ (s1 =~ c1) = true /\ (s2 =~ c2) = true ).
+Proof. induction s.
+- intros c1 c2 H. exists []. exists []. simpl. simpl in H. apply andb_prop in H as [H1 H2].
+  rewrite H1. rewrite H2. split.
+  * reflexivity.
+  * split.
+    ** reflexivity.
+    ** reflexivity.
+- intros c1 c2 H. apply mseq_oper_inv_helper.
+  * unfold exists_seq_decomp_def. intros H2. apply IHs. apply H2.
+  * apply H.
+Qed.
+
+Lemma oper_imp_comp : forall (s : Trace)(c : Contract), (s =~ c) = true -> s ==~ c.
+Proof.
+intros s c. generalize dependent s. induction c.
+- intros s H. destruct s. (*Success*)
+  * apply MSuccess.
+  * inversion H. rewrite failure_false in H1. discriminate H1.
+- intros s H. rewrite failure_false in H. discriminate H. (*Failure*)
+- intros s H. destruct s eqn:Heqn. (*Event e*)
+  * inversion H.
+  * simpl in H. destruct (eq_event_prop e e0). (*reflection*)
+    ** apply success_empty in H. rewrite H0. rewrite H. apply MEvent.
+    ** rewrite failure_false in H. discriminate H.
+- intros s H. apply plus_or_oper in H. destruct H. (*c1 _+_ c2*)
+  * apply MPlusL. apply IHc1. apply H.
+  * apply MPlusR. apply IHc2. apply H.
+- intros s H. apply mseq_oper_inv in H as [s' [s'' [P1 [P2 P3]]]]. (*c1 _;_ c2*)
+  rewrite P1. apply MSeq.
+  * apply (IHc1 s' P2).
+  * apply (IHc2 s'' P3). 
+Qed.
+
+Lemma comp_iff_oper : forall (s : Trace)(c : Contract), s ==~ c <-> (s =~ c) = true.
+Proof.
+split.
+- (*->*) apply comp_imp_oper.
+- (*<-*) apply oper_imp_comp.
+Qed.
+
+(*the boolean value s =~ c is reflected in the proposition s ==~ c *)
+Lemma matches_prop : forall (s : Trace) (c : Contract), reflect (s ==~ c) (s =~ c).
+Proof.
+  intros n m. apply iff_reflect. split.
+- apply comp_iff_oper.
+- apply comp_iff_oper.
+Qed.
+
+
+Definition c_eq (c c':Contract) : Prop := forall s, s ==~ c <-> s ==~ c'.
 Notation "a =R= b" := (c_eq a b) (at level 70).
+
+Definition c_le (c c':Contract) : Prop := forall s, s ==~ c -> s ==~ c'.
+Notation "a <R= b" := (c_le a b) (at level 70).
 
 Lemma c_eq_refl : reflexive Contract c_eq.
 Proof.
-  unfold reflexive. intro x. unfold c_eq. intro s. auto.
+  unfold reflexive. intro x. split.
+- intros H. apply H.
+- intros H. apply H.
 Qed.
 
 Lemma c_eq_sym : symmetric Contract c_eq.
 Proof.
-  unfold symmetric. intros x y. unfold c_eq. intro H. auto.
+  unfold symmetric. intros x y. unfold c_eq. intro H. split.
+- intro H2. apply H. apply H2.
+- intro H2. apply H. apply H2.
 Qed.
 
 
-(*Question: Is transitivity both a proposition and a proof method?*)
 Lemma c_eq_trans: transitive Contract c_eq.
 Proof.
-  unfold transitive.  intros x y z.  unfold c_eq in *. intros Hxy Hyz s.
-  transitivity (y ~= s); auto.
+  unfold transitive.  intros x y z.  unfold c_eq. intros Hxy Hyz s. split.
+- intro H. apply Hyz. apply Hxy. apply H.
+- intro H. apply Hxy. apply Hyz. apply H.
 Qed.
 
 Add Parametric Relation : Contract c_eq
@@ -118,70 +355,90 @@ Add Parametric Relation : Contract c_eq
   transitivity proved by c_eq_trans
   as Contract_setoid.
 
-Definition bool_eq (a a':bool) : Prop := a = a'.
-Definition event_eq (a a':EventType) : Prop := a = a'.
 
-(*nu is morphism from (Contract,c_eq) to (Bool,bool_eq) *)
-Lemma nu_equals : forall c c', c =R= c' -> nu c = nu c'.
+
+Lemma plus_comm_le : forall (c1 c2 : Contract), (c1 _+_ c2) <R= (c2 _+_ c1).
 Proof.
-  unfold c_eq. intros c c' H.
-  specialize (H []%list); simpl in H. auto.
-Qed.
+- intros c1 c2 s H. inversion H.
+  * apply MPlusR. apply H2.
+  * apply MPlusL. apply H1.
+Qed. 
 
-Add Parametric Morphism : nu with
-signature c_eq ==> bool_eq as nu_morphism.
+Lemma plus_comm : forall (c1 c2 : Contract), (c1 _+_ c2) =R= (c2 _+_ c1).
 Proof.
-  intros x y H. apply nu_equals. auto.
+split.
+- apply plus_comm_le.
+- apply plus_comm_le.
 Qed.
 
-(*derive is morphism from (EventType,event_eq) and (Contract,c_eq) to (Contract,c_eq) *)
-Lemma derive_equals : forall c c', c =R= c' -> (forall a, c / a =R= c' / a).
+Lemma plus_assoc : forall (c1 c2 c3 : Contract), ((c1 _+_ c2) _+_ c3) =R= (c1 _+_ (c2 _+_ c3)).
 Proof.
-  intros c c' H. unfold c_eq. intros a s.
-  repeat rewrite <- derivation. auto.
+split.
+- intro H. inversion H.
+  * inversion H2.
+    ** apply MPlusL. apply H6.
+    ** apply MPlusR. apply MPlusL. apply H6.
+  * apply MPlusR. apply MPlusR. apply H1.
+- intro H. inversion H.
+  * inversion H2.
+    ** apply MPlusL. apply MPlusL. apply MSuccess.
+    ** apply MPlusL. apply MPlusL. apply MEvent.
+    ** apply MPlusL. apply MPlusL. apply MSeq.
+      *** apply H4.
+      *** apply H5.
+    ** apply MPlusL. apply MPlusL. apply MPlusL. apply H4.
+    ** apply MPlusL. apply MPlusL. apply MPlusR. apply H4.
+  * inversion H1.
+    ** apply MPlusL. apply MPlusR. apply H6.
+    ** apply MPlusR. apply H6.
 Qed.
 
-Add Parametric Morphism : derive with
-signature event_eq ==> c_eq ==> c_eq as derive_morphism.
+Search (_ ++ _ = _).
+
+Lemma seq_assoc : forall (c1 c2 c3 : Contract), ((c1 _;_ c2) _;_ c3) =R= (c1 _;_ (c2 _;_ c3)).
 Proof.
-  intros x y H. intros x0 y0 H0.
-  inversion H. rewrite <- H1.
-  apply derive_equals. auto.
+split.
+- intro H. inversion H. inversion H3. rewrite <- app_assoc. apply MSeq.
+  * apply H8.
+  * apply MSeq.
+    ** apply H9.
+    ** apply H4.
+- intro H. inversion H. inversion H4. rewrite -> app_assoc. apply MSeq.
+  * apply MSeq.
+    ** apply H3.
+    ** apply H8.
+  * apply H9.
+Qed.
+
+Lemma plus_or : forall (s : Trace)(c1 c2 : Contract), s ==~ (c1 _+_ c2) -> s ==~ c1 \/ s ==~c2.
+Proof. 
+intros s c1 c2 H. repeat rewrite comp_iff_oper in *.
+apply plus_or_oper in H. apply H.
 Qed.
 
 
-  
-(*Example*)
-Example test_1: Success ~== [].
-Proof. unfold matches. reflexivity.
+Lemma plus_distr : forall (c1 c2 c3 : Contract), (c1 _;_ (c2 _+_ c3)) =R= (c1 _;_ c2) _+_ (c1 _;_ c3).
+Proof. split.
+- intro H. inversion H. inversion H4.
+  * apply MPlusL. apply MSeq. { apply H3. } { apply H7. }
+  * apply MPlusR. apply MSeq. { apply H3. } { apply H7. }
+- intro H. apply plus_or in H as [H | H].
+  * inversion H. apply MSeq.
+    ** apply H3.
+    ** apply MPlusL. apply H4.
+  * inversion H. apply MSeq.
+    ** apply H3.
+    ** apply MPlusR. apply H4.
 Qed.
 
-Definition contract2 := Transfer _._ Notify _._ Success
-                       _+_ 
-                        Success _;_ Notify _._ Transfer _._ Success. 
-
-Example test_2_1: contract2 ~== [Transfer; Notify].
-Proof. unfold matches.  reflexivity.
+Lemma plus_distr2 : forall (c1 c2 c3 : Contract), ((c1 _+_ c2) _;_ c3) =R= (c1 _;_ c3) _+_ (c2 _;_ c3).
+Proof. split.
+- intros H. inversion H. inversion H3.
+  * apply MPlusL. apply MSeq. { apply H7. } { apply H4. }
+  * apply MPlusR. apply MSeq. { apply H7. } { apply H4. }
+- intros H. inversion H.
+  * inversion H2. apply MSeq. { apply MPlusL. apply H7. } { apply H8. }
+  * inversion H1. apply MSeq. { apply MPlusR. apply H7. } { apply H8. }
 Qed.
-
-Example test_2_2: contract2 ~== [Notify; Transfer].
-Proof. unfold matches.  reflexivity.
-Qed.
-
-Example test_2_3: contract2 ~!= [Notify; Notify].
-Proof. unfold matches.  reflexivity.
-Qed.
-
-(**)
-
-(*Prove algebraic properties*)
-
-(*Is it interesting to mechanize the denotation of a contract? fx for choice it could be
-  denotation c1 _+_ c2 := forall s : Trace, s in (denotation c1) \/ s in (denotation c2) *)
-
-
-
-
-
 
 
